\begin{dmath*}
Omega = \frac{1-{{\alpha}}}{1-{{\alpha}}+{{\alpha}}\, {{\epsilon_p}}}
\end{dmath*}
\begin{dmath*}
psi\_n\_ya = \frac{1+{{\varphi}}}{{{\alpha}}+{{\varphi}}+\left(1-{{\alpha}}\right)\, {{\sigma}}}
\end{dmath*}
\begin{dmath*}
psi\_n\_wa = \frac{1-{{\alpha}}\, \frac{1+{{\varphi}}}{{{\alpha}}+{{\varphi}}+\left(1-{{\alpha}}\right)\, {{\sigma}}}}{1-{{\alpha}}}
\end{dmath*}
\begin{dmath*}
lambda\_p = \frac{1-{{\alpha}}}{1-{{\alpha}}+{{\alpha}}\, {{\epsilon_p}}}\, \frac{\left(1-{{\theta_p}}\right)\, \left(1-{{\theta_p}}\, {{\beta}}\right)}{{{\theta_p}}}
\end{dmath*}
\begin{dmath*}
aleph\_p = \frac{{{\alpha}}\, \frac{1-{{\alpha}}}{1-{{\alpha}}+{{\alpha}}\, {{\epsilon_p}}}\, \frac{\left(1-{{\theta_p}}\right)\, \left(1-{{\theta_p}}\, {{\beta}}\right)}{{{\theta_p}}}}{1-{{\alpha}}}
\end{dmath*}
\begin{dmath*}
lambda\_w = \frac{\left(1-{{\theta_w}}\right)\, \left(1-{{\beta}}\, {{\theta_w}}\right)}{{{\theta_w}}\, \left(1+{{\varphi}}\, {{\epsilon_w}}\right)}
\end{dmath*}
\begin{dmath*}
aleph\_w = \frac{\left(1-{{\theta_w}}\right)\, \left(1-{{\beta}}\, {{\theta_w}}\right)}{{{\theta_w}}\, \left(1+{{\varphi}}\, {{\epsilon_w}}\right)}\, \left({{\sigma}}+\frac{{{\varphi}}}{1-{{\alpha}}}\right)
\end{dmath*}
% Equation 1
\begin{dmath}
{{\pi^p}}_{t}={{\beta}}\, {{\pi^p}}_{t+1}+{{\tilde y}}_{t}\, \frac{{{\alpha}}\, \frac{1-{{\alpha}}}{1-{{\alpha}}+{{\alpha}}\, {{\epsilon_p}}}\, \frac{\left(1-{{\theta_p}}\right)\, \left(1-{{\theta_p}}\, {{\beta}}\right)}{{{\theta_p}}}}{1-{{\alpha}}}+{{\tilde \omega}}_{t}\, \frac{1-{{\alpha}}}{1-{{\alpha}}+{{\alpha}}\, {{\epsilon_p}}}\, \frac{\left(1-{{\theta_p}}\right)\, \left(1-{{\theta_p}}\, {{\beta}}\right)}{{{\theta_p}}}
\end{dmath}
% Equation 2
\begin{dmath}
{{\pi^w}}_{t}={{\beta}}\, {{\pi^w}}_{t+1}+{{\tilde y}}_{t}\, \frac{\left(1-{{\theta_w}}\right)\, \left(1-{{\beta}}\, {{\theta_w}}\right)}{{{\theta_w}}\, \left(1+{{\varphi}}\, {{\epsilon_w}}\right)}\, \left({{\sigma}}+\frac{{{\varphi}}}{1-{{\alpha}}}\right)-\frac{\left(1-{{\theta_w}}\right)\, \left(1-{{\beta}}\, {{\theta_w}}\right)}{{{\theta_w}}\, \left(1+{{\varphi}}\, {{\epsilon_w}}\right)}\, {{\tilde \omega}}_{t}
\end{dmath}
% Equation 3
\begin{dmath}
{{\tilde y}}_{t}=\frac{\left(-1\right)}{{{\sigma}}}\, \left({{i}}_{t}-{{\pi^p}}_{t+1}-{{r^{nat}}}_{t}\right)+{{\tilde y}}_{t+1}
\end{dmath}
% Equation 4
\begin{dmath}
{{i}}_{t}={{\pi^p}}_{t}\, {{\phi_{\pi}}}+{{\phi_{y}}}\, {{\hat y}}_{t}+{{\nu}}_{t}
\end{dmath}
% Equation 5
\begin{dmath}
{{r^{nat}}}_{t}=\left(1-{{\rho_{z}}}\right)\, {{z}}_{t}+{{a}}_{t}\, \left(1-{{\rho_a}}\right)\, \frac{1+{{\varphi}}}{{{\alpha}}+{{\varphi}}+\left(1-{{\alpha}}\right)\, {{\sigma}}}\, \left(-{{\sigma}}\right)
\end{dmath}
% Equation 6
\begin{dmath}
{{\tilde \omega}}_{t}={{\pi^w}}_{t}+{{\tilde \omega}}_{t-1}-{{\pi^p}}_{t}-\left({{w^{nat}}}_{t}-{{w^{nat}}}_{t-1}\right)
\end{dmath}
% Equation 7
\begin{dmath}
{{w^{nat}}}_{t}={{a}}_{t}\, \frac{1-{{\alpha}}\, \frac{1+{{\varphi}}}{{{\alpha}}+{{\varphi}}+\left(1-{{\alpha}}\right)\, {{\sigma}}}}{1-{{\alpha}}}
\end{dmath}
% Equation 8
\begin{dmath}
{{\mu^p}}_{t}={{\tilde y}}_{t}\, \frac{\left(-{{\alpha}}\right)}{1-{{\alpha}}}-{{\tilde \omega}}_{t}
\end{dmath}
% Equation 9
\begin{dmath}
{{\tilde \omega}}_{t}={\omega}_{t}-{{w^{nat}}}_{t}
\end{dmath}
% Equation 10
\begin{dmath}
{{r^r}}_{t}={{i}}_{t}-{{\pi^p}}_{t+1}
\end{dmath}
% Equation 11
\begin{dmath}
{{y^{nat}}}_{t}=\frac{1+{{\varphi}}}{{{\alpha}}+{{\varphi}}+\left(1-{{\alpha}}\right)\, {{\sigma}}}\, {{a}}_{t}
\end{dmath}
% Equation 12
\begin{dmath}
{{\tilde y}}_{t}={{y}}_{t}-{{y^{nat}}}_{t}
\end{dmath}
% Equation 13
\begin{dmath}
{{\nu}}_{t}={{\rho_{\nu}}}\, {{\nu}}_{t-1}+{{\varepsilon_\nu}}_{t}
\end{dmath}
% Equation 14
\begin{dmath}
{{a}}_{t}={{\rho_a}}\, {{a}}_{t-1}+{{\varepsilon_a}}_{t}
\end{dmath}
% Equation 15
\begin{dmath}
{{y}}_{t}={{a}}_{t}+\left(1-{{\alpha}}\right)\, {{n}}_{t}
\end{dmath}
% Equation 16
\begin{dmath}
{{z}}_{t}={{\rho_{z}}}\, {{z}}_{t-1}-{{\varepsilon_z}}_{t}
\end{dmath}
% Equation 17
\begin{dmath}
{{\Delta m}}_{t}=4\, \left({{\pi^p}}_{t}+{{y}}_{t}-{{y}}_{t-1}-{{\eta}}\, \left({{i}}_{t}-{{i}}_{t-1}\right)\right)
\end{dmath}
% Equation 18
\begin{dmath}
{{(m-p)}}_{t}={{y}}_{t}-{{i}}_{t}\, {{\eta}}
\end{dmath}
% Equation 19
\begin{dmath}
{{i^{ann}}}_{t}={{i}}_{t}\, 4
\end{dmath}
% Equation 20
\begin{dmath}
{{r^{r,ann}}}_{t}={{r^r}}_{t}\, 4
\end{dmath}
% Equation 21
\begin{dmath}
{{r^{nat,ann}}}_{t}={{r^{nat}}}_{t}\, 4
\end{dmath}
% Equation 22
\begin{dmath}
{{\pi^{p,ann}}}_{t}={{\pi^p}}_{t}\, 4
\end{dmath}
% Equation 23
\begin{dmath}
{{\pi^{w,ann}}}_{t}={{\pi^w}}_{t}\, 4
\end{dmath}
% Equation 24
\begin{dmath}
{{\hat y}}_{t}={{y}}_{t}-(\bar{{y}})
\end{dmath}
% Equation 25
\begin{dmath}
{{\pi^p}}_{t}={{p}}_{t}-{{p}}_{t-1}
\end{dmath}
% Equation 26
\begin{dmath}
{{y}}_{t}={{c}}_{t}
\end{dmath}
% Equation 27
\begin{dmath}
{\omega}_{t}={{w}}_{t}-{{p}}_{t}
\end{dmath}
% Equation 28
\begin{dmath}
{{m}}_{t}={{(m-p)}}_{t}+{{p}}_{t}
\end{dmath}
